coqimp/contextswitch/proof/RegRestoreProof.v
@@ -1,4 +1,4 @@
-Require Import Coqlib.                                                                 
+Require Import Coqlib.                                                                  
 Require Import Maps.            
 Require Import LibTactics.   
         
@@ -38,41 +38,37 @@ Open Scope nat.
 Open Scope code_scope.
 Open Scope mem_scope.
 
-Theorem RegSaveProof :
+Theorem RegRestoreProof :
   forall vl,
-    spec |- {{ reg_save_pre vl }}
-             regsave
-           {{ reg_save_post vl }}.
+    spec |- {{ reg_restore_pre vl }}
+             regstore
+           {{ reg_restore_post vl }}.
 Proof.
   intros.
-  unfold reg_save_pre.
-  unfold reg_save_post.
+  unfold reg_restore_pre.
+  unfold reg_restore_post.
   hoare_ex_intro_pre.
+  renames x' to fmg, x'0 to fmo, x'1 to fml, x'2 to fmi.
+  renames x'3 to nctx, x'5 to vy, x'7 to id, x'8 to vi, x'9 to F.
+  renames x'4 to l, x'6 to retl.
   eapply Pure_intro_rule.
   introv Hlgvl.
-  renames x' to fmg, x'0 to fmo, x'1 to fml, x'2 to fmi.
-  renames x'3 to ctx, x'5 to vy, x'7 to id, x'8 to vi, x'9 to F.
-  renames x'4 to l, x'6 to retf.
+  destruct nctx as [nl nctx].
+  destruct nctx as [ [ [rl ri] rg] ry].
   hoare_lift_pre 5.
   eapply Pure_intro_rule.
   introv Hpure.
   destruct Hpure as [Hsp [Hctx_addr Hretf] ].
-  destruct fmg, fmo, fml, fmi.
-  simpl in Hsp.
-  simpl in Hretf.
-  inversion Hsp; subst.
-  inversion Hretf; subst.
-  destruct ctx as [l ctx].
-  simpl get_ctx_addr.
-  destruct ctx as [ [ [rl ri] rg] ry].
+  simpl in Hctx_addr.
+  inversion Hctx_addr; subst.
+  unfold regstore.
   hoare_lift_pre 2.
   unfold context at 1.
-  unfold context' at 1.
+  unfold context'.
   eapply backward_rule.
   introv Hs.
   asrt_to_line_in Hs 3.
   eauto.
-  unfold regsave.
  
   save_reg_unfold.
   hoare_lift_pre 2.
@@ -92,168 +88,149 @@ Proof.
   unfold save_reg at 1 in Hs.
   asrt_to_line_in Hs 4.
   simpl_sep_liftn_in Hs 5.
+  simpl_sep_liftn_in Hs 22.
   eauto.
 
-  Ltac solve_st_ctx :=
+  Ltac solve_ld_ctx :=
     eapply seq_rule;
-    [TimReduce_simpl; eapply st_rule_reg; eauto;
-    try solve [simpl; repeat (rewrite Int.add_assoc); eauto] | simpl get_genreg_val].
+    [TimReduce_simpl; eapply ld_rule_reg; eauto;
+    try solve [simpl; repeat (rewrite Int.add_assoc); eauto] | simpl upd_genreg].
+
+  destruct fmg, fmo, fml, fmi.
+  simpl in Hsp.
+  inversion Hsp; subst.
   
-  (** st l0 (l5 + OS_L0_OFFSET) *)
-  unfold OS_L0_OFFSET.
-  hoare_lift_pre 22.
-  solve_st_ctx.
+  (** ld (l5 + OS_L0_OFFSET) l0 *)
+  solve_ld_ctx.
   simpl.
+  unfold OS_L0_OFFSET.
   rewrite in_range0; eauto.
   rewrite Int.add_zero; eauto.
-
-  (** st l1 (l5 + OS_L1_OFFSET) *)
-  unfold OS_L1_OFFSET.
+ 
+  (** ld (l5 + OS_L1_OFFSET) l1 *)
   hoare_lift_pre 3.
   hoare_lift_pre 2.
-  solve_st_ctx.
+  solve_ld_ctx.
 
-  (** st l2 (l5 + OS_L2_OFFSET) *)
-  unfold OS_L2_OFFSET.
+  (** ld (l5 + OS_L2_OFFSET) l2 *)
   hoare_lift_pre 4.
   hoare_lift_pre 2.
-  solve_st_ctx.
+  solve_ld_ctx.
 
-  (** st l3 (l5 + OS_L3_OFFSET) *)
-  unfold OS_L3_OFFSET.
+  (** ld (l5 + OS_L3_OFFSET) l3 *)
   hoare_lift_pre 5.
   hoare_lift_pre 2.
-  solve_st_ctx.
+  solve_ld_ctx.
 
-  (** st i0 (l5 + OS_I0_OFFSET) *)
-  unfold OS_I0_OFFSET.
+  (** ld (l5 + OS_I0_OFFSET) i0 *)
   hoare_lift_pre 6.
   hoare_lift_pre 2.
-  solve_st_ctx.
+  solve_ld_ctx.
 
-  (** st i1 (l5 + OS_I1_OFFSET) *)
-  unfold OS_I1_OFFSET.
+  (** ld (l5 + OS_I1_OFFSET) i1 *)
   hoare_lift_pre 7.
   hoare_lift_pre 2.
-  solve_st_ctx.
+  solve_ld_ctx.
 
-  (** st i2 (l5 + OS_I2_OFFSET) *)
-  unfold OS_I2_OFFSET.
+  (** ld (l5 + OS_I2_OFFSET) i2 *)
   hoare_lift_pre 8.
   hoare_lift_pre 2.
-  solve_st_ctx.
+  solve_ld_ctx.
 
-  (** st i3 (l5 + OS_I3_OFFSET) *)
-  unfold OS_I3_OFFSET.
+  (** ld (l5 + OS_I3_OFFSET) i3 *)
   hoare_lift_pre 9.
   hoare_lift_pre 2.
-  solve_st_ctx.
+  solve_ld_ctx.
 
-  (** st i4 (l5 + OS_I4_OFFSET) *)
-  unfold OS_I4_OFFSET.
+  (** ld (l5 + OS_I4_OFFSET) i4 *)
   hoare_lift_pre 10.
   hoare_lift_pre 2.
-  solve_st_ctx.
+  solve_ld_ctx.
 
-  (** st i5 (l5 + OS_I5_OFFSET) *)
-  unfold OS_I5_OFFSET.
+  (** ld (l5 + OS_I5_OFFSET) i5 *)
   hoare_lift_pre 11.
   hoare_lift_pre 2.
-  solve_st_ctx.
+  solve_ld_ctx.
 
-  (** st i6 (l5 + OS_I6_OFFSET) *)
-  unfold OS_I6_OFFSET.
+  (** ld (l5 + OS_I6_OFFSET) i6 *)
   hoare_lift_pre 12.
   hoare_lift_pre 2.
-  solve_st_ctx.
+  solve_ld_ctx.
 
-  (** st i7 (l5 + OS_I7_OFFSET) *)
-  unfold OS_I2_OFFSET.
+  (** ld (l5 + OS_I7_OFFSET) i7 *)
   hoare_lift_pre 13.
   hoare_lift_pre 2.
-  solve_st_ctx.
+  solve_ld_ctx.
 
-  (** rd y l6 *)
+  (** ld (l5 + OS_Y_OFFSET) l6 *)
+  hoare_lift_pre 22.
+  hoare_lift_pre 2.
+  solve_ld_ctx.
+
+  (** wr l6 0 Ry *)
   hoare_lift_pre 23.
   hoare_lift_pre 2.
   eapply seq_rule.
   TimReduce_simpl.
-  eapply rd_rule_reg; eauto.
-  simpl upd_genreg.
+  eapply wr_rule_reg; eauto.
+  simpl; eauto.
+  rewrite in_range0; eauto.
+  simpl set_spec_reg.
+  rewrite Int.xor_zero.
 
-  (** st l6 (l5 + OS_Y_OFFSET) *)
-  hoare_lift_pre 23.
-  hoare_lift_pre 2.
-  solve_st_ctx.
-
-  (** st g1 (l5 + OS_G1_OFFSET) *)
-  unfold OS_G1_OFFSET. 
+  (** ld (l5 + OS_G1_OFFSET) g1 *)
   hoare_lift_pre 17.
   hoare_lift_pre 2.
-  solve_st_ctx.
+  solve_ld_ctx.
 
-  (** st g2 (l5 + OS_G2_OFFSET) *)
-  unfold OS_G2_OFFSET. 
+  (** ld (l5 + OS_G2_OFFSET) g2 *)
   hoare_lift_pre 18.
   hoare_lift_pre 2.
-  solve_st_ctx.
+  solve_ld_ctx.
 
-  (** st g3 (l5 + OS_G3_OFFSET) *)
-  unfold OS_G3_OFFSET. 
+  (** ld (l5 + OS_G3_OFFSET) g3 *)
   hoare_lift_pre 19.
   hoare_lift_pre 2.
-  solve_st_ctx.
+  solve_ld_ctx.
 
-  (** st g4 (l5 + OS_G4_OFFSET) *)
-  unfold OS_G4_OFFSET. 
+  (** ld (l5 + OS_G4_OFFSET) g4 *)
   hoare_lift_pre 20.
   hoare_lift_pre 2.
-  solve_st_ctx.
- 
-  (** st g5 (l5 + OS_G5_OFFSET) *)
-  unfold OS_G5_OFFSET. 
+  solve_ld_ctx.
+
+  (** ld (l5 + OS_G5_OFFSET) g5 *)
   hoare_lift_pre 21.
   hoare_lift_pre 2.
-  solve_st_ctx.
+  solve_ld_ctx.
 
-  (** st g6 (l5 + OS_G6_OFFSET) *)
-  unfold OS_G6_OFFSET. 
+  (** ld (l5 + OS_G6_OFFSET) g6 *)
   hoare_lift_pre 22.
   hoare_lift_pre 2.
-  solve_st_ctx.
+  solve_ld_ctx.
 
-  (** st g7 (l5 + OS_G7_OFFSET) *)
-  unfold OS_G7_OFFSET. 
+  (** ld (l5 + OS_G7_OFFSET) g7 *)
   hoare_lift_pre 23.
   hoare_lift_pre 2.
-  solve_st_ctx.
+  solve_ld_ctx.
 
+  (** retl; nop *)
   eapply retl_rule; eauto.
   TimReduce_simpl.
   eapply nop_rule; eauto.
   introv Hs.
   sep_ex_intro.
   eapply sep_pure_l_intro; eauto.
-  simpl update_frame.
-  sep_cancel1 1 1. 
-  instantiate (1 :=
-                 (l, (w15 :: w16 :: w17 :: w18 :: nil,
-                      w23 :: w24 :: w25 :: w26 :: w27 :: w28 :: w29 :: w30 :: nil,
-                      a11 :: w0 :: w1 :: w2 :: w3 :: w4 :: w5 :: w6 :: nil, vy))
-              ).
-  sep_cancel1 9 2.
-  sep_cancel1 22 2.
+  sep_cancel1 1 1.
+  sep_cancel1 8 2.
   unfold context, context'.
-  asrt_to_line 3.
-  unfold save_reg at 1.
+  asrt_to_line 4.
+  unfold save_reg.
   asrt_to_line 4.
   simpl_sep_liftn 5.
   simpl_sep_liftn 5.
-  unfold save_reg at 1.
   asrt_to_line 8.
   simpl_sep_liftn 9.
   simpl_sep_liftn 13.
-  unfold save_reg at 1.
   asrt_to_line 8.
   simpl_sep_liftn 9.
 
@@ -278,35 +255,38 @@ Proof.
   sep_cancel1 1 3.
   sep_cancel1 1 2.
   sep_cancel1 1 1.
+  sep_cancel1 1 1.
   instantiate (1 := Aemp).
   eapply astar_emp_intro_r; eauto.
-
   eapply astar_emp_elim_r.
   eapply sep_pure_l_intro; eauto.
-  simpl.
+  simpls.
   repeat (split; eauto).
 
   unfold fretSta.
   TimReduce_simpl.
   introv Hs Hs'.
-  destruct_state s.
-  destruct_state s'.
-  eapply getR_eq_get_genreg_val1 with (rr := r15) in Hs.
-  simpl get_genreg_val in Hs.
+  simpl in Hretf.
+  inversion Hretf; subst.
   sep_ex_elim_in Hs'.
   eapply sep_pure_l_elim in Hs'.
   destruct Hs' as [Hlgvl1 Hs'].
   inversion Hlgvl1; subst.
-  simpl update_frame in Hs'.
-  eapply getR_eq_get_genreg_val1 with (rr := r15) in Hs'.
-  simpl get_genreg_val in Hs'.
-  simpl.
-  clear - Hs Hs'.
+  destruct x, x0, x1, x2.
+  simpl_sep_liftn_in Hs' 5.
+  eapply sep_pure_l_elim in Hs'.
+  destruct Hs' as [Hctx_win_restore Hs'].
+  destruct_state s.
+  destruct_state s'.
+  eapply getR_eq_get_genreg_val1 with (rr := r15) in Hs; eauto.
+  eapply getR_eq_get_genreg_val1 with (rr := r15) in Hs'; eauto.
+  clear - Hs Hctx_win_restore Hs'.
+  simpls.
+  simpljoin1.
   unfolds get_R.
   destruct (r r15); tryfalse.
-  inversion Hs; subst.
   destruct (r0 r15); tryfalse.
-  inversion Hs'; subst.
+  inversion H0; subst.
   eauto.
 Qed.
 
